


\documentclass[11pt]{article}
\usepackage{fullpage}
\usepackage{amsthm}
\usepackage{amsthm,amsmath,amsfonts,amssymb,amstext}
\usepackage{latexsym,ifthen,url,rotating}
\usepackage[usenames,dvipsnames]{color}


% --- -----------------------------------------------------------------
% --- Document-specific definitions.
% --- -----------------------------------------------------------------
\newtheorem{definition}{Definition}

\newcommand{\concat}{{\,\|\,}}
\newcommand{\bits}{\{0,1\}}
\newcommand{\Range}{{\mathrm{Range}}}
\newcommand{\A}{{\mathcal{A}}}

% --- -----------------------------------------------------------------
% --- The document starts here.
% --- -----------------------------------------------------------------
\begin{document}
%\maketitle
\sloppy

\noindent Paul Jones \\
Rutgers University\\
CS206: Introduction to Discrete Structures II, Spring 2013\\
Professor David Cash\\

\begin{center}
Homework 8
\end{center}

\begin{enumerate}

\item (7 points each) Solve the following recurrences using generating
functions.  Show all of your work.  Solutions without detailed
explanations will receive little or no credit.
\begin{enumerate}
	\item $a_0 = 1, a_1=1$, and for $n \geq 2$, $a_n = a_{n-1} + 2a_{n-2}$

	\[ a(x) = \sum a_n x^n \]
	\[ a_n = a_{n - 1} + 2a_{n - 2} = 0 \]
	\[ \sum_{n = 2}^{\infty} \left(x^n a_{n - 1} + 2 x^n a_{n - 2} \right) = 0 \]
	\[ \sum_{n = 2}^{\infty} x^n a_{n - 1} + 2 \sum_{n = 2}^{\infty} x^n a_{n - 2} = 0 \]
	\[ x \sum_{n = 2}^{\infty} x^{n - 1} a_{n - 1} + 2 x^2 \sum_{n = 2}^{\infty} x^{n - 2} a_{n - 2} = 0 \]	
	\[ x (a(x) - a(0)) + 2 x^2 a(x) = 0 \]
	\[ x (a(x) - 1) + 2 x^2 a(x)  = 0\]	
	\[ x a(x) - x + 2 x^2 a(x) = 0\]
	\[ x a(x) + 2 x^2 a(x) = x\]
	\[ a(x) (x + 2 x^2) = x\]
	\[ a(x) = \frac{x}{x + 2 x^2}\]	
	\[ a(x) = \frac{1}{1 + 2 x}\]	

	\clearpage

	\item $a_0 = 1, a_1=1$, and for $n\geq 2$, $a_n = a_{n-1} + 2 a_{n-2} + 4$

	\[ a(x) = \sum a_n x^n \]
	\[ a_n = a_{n-1} + 2 a_{n-2} + 4 = 0 \]
	\[ \sum_{n = 2}^{\infty} \left(x^n a_{n - 1} + 2 x^n a_{n - 2} + 4 x^n\right) = 0 \]
	\[ x \sum_{n = 2}^{\infty} x^{n - 1} a_{n - 1} + 2x^2 \sum_{n = 2}^{\infty} x^{n - 2} a_{n - 2} + 4 \sum_{n = 2}^{\infty} x^n = 0 \]
	\[ x (a(x) - a(0)) + 2x^2 a(x) + 4 \sum_{n = 2}^{\infty} x^n = 0 \]
	\[ x (a(x) - a(0)) + 2x^2 a(x) + \frac{4}{1 - x} = 0 \]
	\[ x (a(x) - 1) + 2x^2 a(x) + \frac{4}{1 - x} = 0 \]

	\clearpage

	\item $a_0 = 1$, and for $n\geq 1$, $a_n = 3a_{n-1} + 4^{n-1}$

	\[ a(x) = \sum a_n x^n \]
	\[ a_n = 3a_{n-1} + 4^{n-1} = 0\]
	\[ \sum_{n = 1}^\infty x^n a_{n-1} + \sum_{n = 1}^\infty x^n 4^{n-1} = 0\]
	\[ x \sum_{n = 1}^\infty x^{n -1} a_{n-1} + \frac{1}{4} \sum_{n = 1}^\infty x^n 4^{n} = 0 \]
	\[ x (a(x) - a(0)) + \frac{1}{4} \frac{1}{1 - 4x} = 0 \]
	\[ x (a(x) - 1) + \frac{1}{4(1 - 4x)} = 0 \]

\end{enumerate}
\end{enumerate}
\end{document}

